coq/soundness.v
@@ -1,7 +1,0 @@
-Require Export lc.tactics.
-Require Export lc.relations.
-Require Import Lia.
-Require Import Coq.Logic.FunctionalExtensionality.
-
-Import LCNotations.
-Local Open Scope lc_scope.
